src/cbor/CBOR.Spec.fst
@@ -19,3 +19,29 @@ let serialize_cbor_nonempty
 = ()
 
 let deterministically_encoded_cbor_map_key_order = CBOR.Spec.Format.deterministically_encoded_cbor_map_key_order
+
+let rec list_ghost_assoc_eq
+  (#key #value: Type)
+  (k: key)
+  (m: list (key & value))
+: Lemma
+  (list_ghost_assoc k m == LowParse.Spec.Assoc.list_ghost_assoc k m)
+  [SMTPat (list_ghost_assoc k m)]
+= match m with
+  | [] -> ()
+  | (k', _) :: m' ->
+    if FStar.StrongExcludedMiddle.strong_excluded_middle (k == k')
+    then ()
+    else list_ghost_assoc_eq k m'
+
+let deterministically_encoded_cbor_map_key_order_assoc_ext
+  m1 m2 ext
+= CBOR.Spec.Format.deterministically_encoded_cbor_map_key_order_assoc_ext m1 m2 ext
+
+let deterministically_encoded_cbor_map_key_order_major_type_intro
+  v1 v2
+= CBOR.Spec.Format.deterministically_encoded_cbor_map_key_order_major_type_intro v1 v2
+
+let deterministically_encoded_cbor_map_key_order_int64
+  ty v1 v2
+= CBOR.Spec.Format.lex_order_int64_correct ty v1 v2
